Update seq.dfy

seq.dfy
@@ -1,6 +1,6 @@
 predicate esteSolutieValida(solutie : seq<int>)
 {
-  |solutie| == 4 && solutie[0]>=0 && solutie[1]>=0 && solutie[2]>=0 && solutie[3]>=0
+  |solutie| == 5 && solutie[0]>=0 && solutie[1]>=0 && solutie[2]>=0 && solutie[3]>=0 && solutie[4]>=0
 }
 
 
@@ -8,7 +8,7 @@ predicate esteSolutieValida(solutie : seq<int>)
 predicate esteSolutie(solutie : seq<int>, nr:int)
   requires esteSolutieValida(solutie)
 {
-    solutie[0]*1+solutie[1]*5+solutie[2]*10+solutie[3]*20 == nr
+    solutie[0]*1+solutie[1]*5+solutie[2]*10+solutie[3]*20+solutie[4]*50 == nr
 
 }
 
@@ -16,7 +16,7 @@ predicate esteSolutie(solutie : seq<int>, nr:int)
 function cost(solutie : seq<int>):int 
   requires esteSolutieValida(solutie)
 {
-    solutie[0]+solutie[1]+solutie[2]+solutie[3]
+    solutie[0]+solutie[1]+solutie[2]+solutie[3]+solutie[4]
 }
 
 predicate esteSolutieOptima(solutie : seq<int>, nr:int)
@@ -34,23 +34,28 @@ predicate INV(copie: int, nr: int, solutieFinala : seq<int>)
    forall solutieCurenta :: esteSolutieValida(solutieCurenta) ==>
           (esteSolutie(solutieCurenta,copie) ==> 
           esteSolutie([solutieFinala[0]+solutieCurenta[0],solutieFinala[1]+solutieCurenta[1],
-          solutieFinala[2]+solutieCurenta[2],solutieFinala[3]+solutieCurenta[3]],nr)) &&
+          solutieFinala[2]+solutieCurenta[2],solutieFinala[3]+solutieCurenta[3],solutieFinala[4]+solutieCurenta[4]],nr)) &&
           (esteSolutieOptima(solutieCurenta,copie) ==> 
           esteSolutieOptima([solutieFinala[0]+solutieCurenta[0],solutieFinala[1]+solutieCurenta[1],
-          solutieFinala[2]+solutieCurenta[2],solutieFinala[3]+solutieCurenta[3]],nr))
+          solutieFinala[2]+solutieCurenta[2],solutieFinala[3]+solutieCurenta[3],solutieFinala[4]+solutieCurenta[4]],nr))
 }
 
 
 method gasireMaxim(nr: int) returns(s:int)
   requires nr > 0
   ensures 0 < s <= nr
-  ensures s == 1 || s == 5 || s == 10 || s == 20
+  ensures s == 1 || s == 5 || s == 10 || s == 20 || s == 50
   ensures s == 1 ==> nr < 5
   ensures s == 5 ==> 5 <= nr < 10
   ensures s == 10 ==> 10 <= nr < 20
-  ensures s == 20 ==> nr >= 20
+  ensures s == 20 ==> 20 <= nr < 50
+  ensures s == 50 ==> nr >= 50
 {
-    if(nr >= 20)
+    if(nr >= 50)
+    {
+        s := 50 ;
+    }
+    else if(nr >= 20)
     {
         s := 20;
     }
@@ -71,31 +76,31 @@ lemma cazMaxim1(copie: int, nr: int, solutieFinala: seq<int>)
   requires copie < 5
   requires esteSolutieValida(solutieFinala)
   requires INV(copie,nr,solutieFinala)
-  ensures INV(copie-1,nr,[(solutieFinala[0]+1),solutieFinala[1],solutieFinala[2],solutieFinala[3]])
+  ensures INV(copie-1,nr,[(solutieFinala[0]+1),solutieFinala[1],solutieFinala[2],solutieFinala[3],solutieFinala[4]])
 {
 
   forall solutieCurenta | esteSolutieValida(solutieCurenta) && esteSolutieOptima(solutieCurenta,copie-1) 
           ensures esteSolutieOptima([solutieFinala[0]+solutieCurenta[0]+1,solutieFinala[1]+solutieCurenta[1],
-          solutieFinala[2]+solutieCurenta[2],solutieFinala[3]+solutieCurenta[3]],nr)
+          solutieFinala[2]+solutieCurenta[2],solutieFinala[3]+solutieCurenta[3],solutieFinala[4]+solutieCurenta[4]],nr)
   {
     assert esteSolutie(solutieCurenta,copie-1);
-    assert esteSolutie([solutieCurenta[0]+1,solutieCurenta[1],solutieCurenta[2],solutieCurenta[3]],copie);
+    assert esteSolutie([solutieCurenta[0]+1,solutieCurenta[1],solutieCurenta[2],solutieCurenta[3],solutieCurenta[4]],copie);
 
     assert forall solutieOarecare :: esteSolutieValida(solutieOarecare) && esteSolutie(solutieOarecare,copie-1) 
           ==> cost(solutieOarecare) >= cost(solutieCurenta);
 
     assert esteSolutie([solutieFinala[0]+solutieCurenta[0]+1,solutieFinala[1]+solutieCurenta[1],
-          solutieFinala[2]+solutieCurenta[2],solutieFinala[3]+solutieCurenta[3]],nr);
+          solutieFinala[2]+solutieCurenta[2],solutieFinala[3]+solutieCurenta[3],solutieFinala[4]+solutieCurenta[4]],nr);
 
     assert forall solutieOarecare :: esteSolutieValida(solutieOarecare) &&  esteSolutie(solutieOarecare,nr) 
           ==> cost(solutieOarecare) >= cost([solutieCurenta[0]+solutieFinala[0]+1,solutieCurenta[1]+solutieFinala[1],
-          solutieCurenta[2]+solutieFinala[2],solutieCurenta[3]+solutieFinala[3]]);
+          solutieCurenta[2]+solutieFinala[2],solutieCurenta[3]+solutieFinala[3],solutieCurenta[4]+solutieFinala[4]]);
   }
 
   assert forall solutieCurenta :: esteSolutieValida(solutieCurenta) 
           && esteSolutieOptima(solutieCurenta,copie-1) ==> 
           esteSolutieOptima([solutieFinala[0]+solutieCurenta[0]+1,solutieFinala[1]+solutieCurenta[1],
-          solutieFinala[2]+solutieCurenta[2],solutieFinala[3]+solutieCurenta[3]],nr);
+          solutieFinala[2]+solutieCurenta[2],solutieFinala[3]+solutieCurenta[3],solutieFinala[4]+solutieCurenta[4]],nr);
 
 }
 
@@ -103,26 +108,29 @@ lemma cazMaxim5(copie: int, nr: int, solutieFinala: seq<int>)
   requires 5 <= copie < 10 
   requires esteSolutieValida(solutieFinala)
   requires INV(copie,nr,solutieFinala)
-  ensures INV(copie-5,nr,[solutieFinala[0],(solutieFinala[1]+1),solutieFinala[2],solutieFinala[3]])
+  ensures INV(copie-5,nr,[solutieFinala[0],(solutieFinala[1]+1),solutieFinala[2],solutieFinala[3],solutieFinala[4]])
 {
 
  forall solutieCurenta | esteSolutieValida(solutieCurenta) && esteSolutieOptima(solutieCurenta,copie-5) 
           ensures esteSolutieOptima([solutieFinala[0]+solutieCurenta[0],solutieFinala[1]+solutieCurenta[1]+1,
-          solutieCurenta[2]+solutieFinala[2],solutieCurenta[3]+solutieFinala[3]],nr)
+          solutieCurenta[2]+solutieFinala[2],solutieCurenta[3]+solutieFinala[3],solutieFinala[4]],nr)
   {
     assert esteSolutie(solutieCurenta,copie-5);
-    assert esteSolutie([solutieCurenta[0], solutieCurenta[1]+1,solutieCurenta[2],solutieCurenta[3]],copie);
+    assert esteSolutie([solutieCurenta[0], solutieCurenta[1]+1,solutieCurenta[2],solutieCurenta[3],solutieCurenta[4]],copie);
 
     assert forall solutieOarecare :: esteSolutieValida(solutieOarecare)  && esteSolutie(solutieOarecare,copie-5) 
           ==> cost(solutieOarecare) >= cost(solutieCurenta);
-    assert esteSolutie([solutieFinala[0]+solutieCurenta[0],solutieFinala[1]+solutieCurenta[1]+1,solutieFinala[2]+solutieCurenta[2],solutieFinala[3]+solutieCurenta[3]],nr);
+    assert esteSolutie([solutieFinala[0]+solutieCurenta[0],solutieFinala[1]+solutieCurenta[1]+1,
+    solutieFinala[2]+solutieCurenta[2],solutieFinala[3]+solutieCurenta[3],solutieFinala[4]+solutieCurenta[4]],nr);
     
     assert forall solutieOarecare :: esteSolutieValida(solutieOarecare) && esteSolutie(solutieOarecare,nr)
-          ==> cost(solutieOarecare) >= cost([solutieFinala[0]+solutieCurenta[0],solutieFinala[1]+solutieCurenta[1]+1,solutieFinala[2]+solutieCurenta[2],solutieFinala[3]+solutieCurenta[3]]);
+          ==> cost(solutieOarecare) >= cost([solutieFinala[0]+solutieCurenta[0],solutieFinala[1]+solutieCurenta[1]+1,
+          solutieFinala[2]+solutieCurenta[2],solutieFinala[3]+solutieCurenta[3],solutieFinala[4]+solutieCurenta[4]]);
   }
 
   assert forall solutieCurenta :: esteSolutieValida(solutieCurenta) && esteSolutie(solutieCurenta,copie-5) ==> 
-          esteSolutieOptima([solutieCurenta[0]+solutieFinala[0],solutieCurenta[1]+solutieFinala[1]+1,solutieCurenta[2]+solutieFinala[2],solutieCurenta[3]+solutieFinala[3]],nr);
+          esteSolutieOptima([solutieCurenta[0]+solutieFinala[0],solutieCurenta[1]+solutieFinala[1]+1,
+          solutieCurenta[2]+solutieFinala[2],solutieCurenta[3]+solutieFinala[3],solutieCurenta[4]+solutieFinala[4]],nr);
 
 }
 
@@ -130,44 +138,45 @@ lemma aux2(copie:int,solutieCurenta:seq<int>)
   requires 10 <= copie < 20
   requires esteSolutieValida(solutieCurenta)
   requires esteSolutieOptima(solutieCurenta,copie-10)
-  ensures esteSolutieOptima([solutieCurenta[0], solutieCurenta[1],solutieCurenta[2]+1,solutieCurenta[3]],copie)
+  ensures esteSolutieOptima([solutieCurenta[0], solutieCurenta[1],solutieCurenta[2]+1,solutieCurenta[3],solutieCurenta[4]],copie)
 {
 
-    assert esteSolutie([solutieCurenta[0], solutieCurenta[1],solutieCurenta[2]+1,solutieCurenta[3]],copie);
-    if(!esteSolutieOptima([solutieCurenta[0], solutieCurenta[1],solutieCurenta[2]+1,solutieCurenta[3]],copie))
+    assert esteSolutie([solutieCurenta[0], solutieCurenta[1],solutieCurenta[2]+1,solutieCurenta[3],solutieCurenta[4]],copie);
+    if(!esteSolutieOptima([solutieCurenta[0], solutieCurenta[1],solutieCurenta[2]+1,solutieCurenta[3],solutieCurenta[4]],copie))
     {
-      var solopt :|esteSolutieValida(solopt) && esteSolutie(solopt,copie) && cost(solopt)<cost([solutieCurenta[0], solutieCurenta[1],solutieCurenta[2]+1,solutieCurenta[3]]);
-      assert cost([solutieCurenta[0], solutieCurenta[1],solutieCurenta[2]+1,solutieCurenta[3]]) == cost(solutieCurenta)+1;
-      assert solopt[3]==0;
-      if(solopt[2]>=1)
+      var solutieOptima :|esteSolutieValida(solutieOptima) && esteSolutie(solutieOptima,copie) && cost(solutieOptima)<cost([solutieCurenta[0], solutieCurenta[1],solutieCurenta[2]+1,solutieCurenta[3],solutieCurenta[4]]);
+      assert cost([solutieCurenta[0], solutieCurenta[1],solutieCurenta[2]+1,solutieCurenta[3],solutieCurenta[4]]) == cost(solutieCurenta)+1;
+      assert solutieOptima[3] == 0;
+      assert solutieOptima[4] == 0;
+      if(solutieOptima[2]>=1)
       {
-        var solopt' := [solopt[0],solopt[1],solopt[2]-1,solopt[3]];
-        assert esteSolutie(solopt',copie-10);
-        assert cost(solopt') == cost(solopt)-1;
-        assert cost(solopt)-1 < cost(solutieCurenta);
+        var solutieOptima' := [solutieOptima[0],solutieOptima[1],solutieOptima[2]-1,solutieOptima[3],solutieOptima[4]];
+        assert esteSolutie(solutieOptima',copie-10);
+        assert cost(solutieOptima') == cost(solutieOptima)-1;
+        assert cost(solutieOptima)-1 < cost(solutieCurenta);
         assert false;
       }
-      else if(solopt[1]>=2)
+      else if(solutieOptima[1]>=2)
       {
-        var solopt' := [solopt[0],solopt[1]-2,solopt[2],solopt[3]];
-        assert esteSolutie(solopt',copie-10);
-        assert cost(solopt') == cost(solopt)-2;
-        assert cost(solopt)-2 < cost(solutieCurenta);
+        var solutieOptima' := [solutieOptima[0],solutieOptima[1]-2,solutieOptima[2],solutieOptima[3],solutieOptima[4]];
+        assert esteSolutie(solutieOptima',copie-10);
+        assert cost(solutieOptima') == cost(solutieOptima)-2;
+        assert cost(solutieOptima)-2 < cost(solutieCurenta);
         assert false;
-      }else if(solopt[1]>=1 && solopt[0]>=5 )
+      }else if(solutieOptima[1]>=1 && solutieOptima[0]>=5 )
       {
-        var solopt' := [solopt[0]-5,solopt[1]-1,solopt[2],solopt[3]];
-        assert esteSolutie(solopt',copie-10);
-        assert cost(solopt') == cost(solopt)-6;
-        assert cost(solopt)-6 < cost(solutieCurenta);
+        var solutieOptima' := [solutieOptima[0]-5,solutieOptima[1]-1,solutieOptima[2],solutieOptima[3],solutieOptima[4]];
+        assert esteSolutie(solutieOptima',copie-10);
+        assert cost(solutieOptima') == cost(solutieOptima)-6;
+        assert cost(solutieOptima)-6 < cost(solutieCurenta);
         assert false;
       }
-      else if(solopt[0]>=10 )
+      else if(solutieOptima[0]>=10 )
       {
-        var solopt' := [solopt[0]-10,solopt[1],solopt[2],solopt[3]];
-        assert esteSolutie(solopt',copie-10);
-        assert cost(solopt') == cost(solopt)-10;
-        assert cost(solopt)-10 < cost(solutieCurenta);
+        var solutieOptima' := [solutieOptima[0]-10,solutieOptima[1],solutieOptima[2],solutieOptima[3],solutieOptima[4]];
+        assert esteSolutie(solutieOptima',copie-10);
+        assert cost(solutieOptima') == cost(solutieOptima)-10;
+        assert cost(solutieOptima)-10 < cost(solutieCurenta);
         assert false;
       }
       else{
@@ -184,117 +193,566 @@ lemma cazMaxim10(copie: int, nr: int, solutieFinala: seq<int>)
   requires 10 <= copie < 20 
   requires esteSolutieValida(solutieFinala) 
   requires INV(copie,nr,solutieFinala)
-  ensures INV(copie-10,nr,[solutieFinala[0],solutieFinala[1],solutieFinala[2]+1,solutieFinala[3]])
+  ensures INV(copie-10,nr,[solutieFinala[0],solutieFinala[1],solutieFinala[2]+1,solutieFinala[3],solutieFinala[4]])
 {
 
  forall solutieCurenta | esteSolutieValida(solutieCurenta) && esteSolutieOptima(solutieCurenta,copie-10) 
           ensures esteSolutieOptima([solutieFinala[0]+solutieCurenta[0],solutieFinala[1]+solutieCurenta[1],
-          solutieCurenta[2]+solutieFinala[2]+1,solutieCurenta[3]+solutieFinala[3]],nr)
+          solutieCurenta[2]+solutieFinala[2]+1,solutieCurenta[3]+solutieFinala[3],solutieCurenta[4]+solutieFinala[4]],nr)
   {
     assert esteSolutie(solutieCurenta,copie-10);
-    assert esteSolutie([solutieCurenta[0], solutieCurenta[1],solutieCurenta[2]+1,solutieCurenta[3]],copie);
+    assert esteSolutie([solutieCurenta[0], solutieCurenta[1],solutieCurenta[2]+1,solutieCurenta[3],solutieCurenta[4]],copie);
 
     aux2(copie,solutieCurenta);
 
-    assert esteSolutieOptima([solutieCurenta[0], solutieCurenta[1],solutieCurenta[2]+1,solutieCurenta[3]],copie);
+    assert esteSolutieOptima([solutieCurenta[0], solutieCurenta[1],solutieCurenta[2]+1,solutieCurenta[3],solutieCurenta[4]],copie);
 
     assert forall solutieOarecare :: esteSolutieValida(solutieOarecare)  && esteSolutie(solutieOarecare,copie-10) 
           ==> cost(solutieOarecare) >= cost(solutieCurenta);
     
 
-    assert esteSolutie([solutieFinala[0]+solutieCurenta[0],solutieFinala[1]+solutieCurenta[1],1+solutieFinala[2]+solutieCurenta[2],solutieFinala[3]+solutieCurenta[3]],nr);
+    assert esteSolutie([solutieFinala[0]+solutieCurenta[0],solutieFinala[1]+solutieCurenta[1],1+solutieFinala[2]+solutieCurenta[2],solutieFinala[3]+solutieCurenta[3],solutieFinala[4]+solutieCurenta[4]],nr);
 
     assert forall solutieOarecare :: esteSolutieValida(solutieOarecare) && esteSolutie(solutieOarecare,nr)
           ==> cost(solutieOarecare) >= cost([solutieCurenta[0]+solutieFinala[0],solutieCurenta[1]+solutieFinala[1],
-                                        solutieCurenta[2]+solutieFinala[2]+1,solutieCurenta[3]+solutieFinala[3]]);
+                                        solutieCurenta[2]+solutieFinala[2]+1,solutieCurenta[3]+solutieFinala[3],solutieCurenta[4]+solutieFinala[4]]);
   }
 
   assert forall solutieCurenta :: esteSolutieValida(solutieCurenta) && esteSolutieOptima(solutieCurenta,copie-10) ==> 
           esteSolutieOptima([solutieCurenta[0]+solutieFinala[0],solutieCurenta[1]+solutieFinala[1],
-                            solutieCurenta[2]+solutieFinala[2]+1,solutieCurenta[3]+solutieFinala[3]],nr);
+                            solutieCurenta[2]+solutieFinala[2]+1,solutieCurenta[3]+solutieFinala[3],solutieCurenta[4]+solutieFinala[4]],nr);
 
 }
+
+
+
+lemma aux3(copie:int,solutieCurenta:seq<int>)
+  requires 20 <= copie < 50
+  requires esteSolutieValida(solutieCurenta)
+  requires esteSolutieOptima(solutieCurenta,copie-20)
+  ensures esteSolutieOptima([solutieCurenta[0], solutieCurenta[1],solutieCurenta[2],1+solutieCurenta[3],solutieCurenta[4]],copie)
+{
+
+    assert esteSolutie([solutieCurenta[0], solutieCurenta[1],solutieCurenta[2],1+solutieCurenta[3],solutieCurenta[4]],copie);
+    if(!esteSolutieOptima([solutieCurenta[0], solutieCurenta[1],solutieCurenta[2],1+solutieCurenta[3],solutieCurenta[4]],copie))
+    {
+      var solutieOptima :|esteSolutieValida(solutieOptima) && esteSolutie(solutieOptima,copie) && cost(solutieOptima)<cost([solutieCurenta[0], solutieCurenta[1],solutieCurenta[2],1+solutieCurenta[3],solutieCurenta[4]]);
+      assert cost([solutieCurenta[0], solutieCurenta[1],solutieCurenta[2],1+solutieCurenta[3],solutieCurenta[4]]) == cost(solutieCurenta)+1;
+      assert solutieOptima[4] == 0;
+      if(solutieOptima[3]>=1)
+      {
+        var solutieOptima' := [solutieOptima[0],solutieOptima[1],solutieOptima[2],solutieOptima[3]-1,solutieOptima[4]];
+        assert esteSolutie(solutieOptima',copie-20);
+        assert cost(solutieOptima') == cost(solutieOptima)-1;
+        assert cost(solutieOptima)-1 < cost(solutieCurenta);
+        assert false;
+      }
+      else if(solutieOptima[2]>=2)
+      {
+        var solutieOptima' := [solutieOptima[0],solutieOptima[1],solutieOptima[2]-2,solutieOptima[3],solutieOptima[4]];
+        assert esteSolutie(solutieOptima',copie-20);
+        assert cost(solutieOptima') == cost(solutieOptima)-2;
+        assert cost(solutieOptima)-2 < cost(solutieCurenta);
+        assert false;
+      }
+      else if(solutieOptima[2]>=1 && solutieOptima[1]>=2)
+      {       
+        var solutieOptima' := [solutieOptima[0],solutieOptima[1]-2,solutieOptima[2]-1,solutieOptima[3],solutieOptima[4]];
+        assert esteSolutie(solutieOptima',copie-20);
+        assert cost(solutieOptima') == cost(solutieOptima)-3;
+        assert cost(solutieOptima)-3 < cost(solutieCurenta);
+        assert false;
+      }
+      else if(solutieOptima[2]>=1 && solutieOptima[1]>=1 && solutieOptima[0]>=5)
+      {
+        var solutieOptima' := [solutieOptima[0]-5,solutieOptima[1]-1,solutieOptima[2]-1,solutieOptima[3],solutieOptima[4]];
+        assert esteSolutie(solutieOptima',copie-20);
+        assert cost(solutieOptima') == cost(solutieOptima)-7;
+        assert cost(solutieOptima)-7 < cost(solutieCurenta);
+        assert false;
+      }
+      else if(solutieOptima[1]>=4)
+      {
+        var solutieOptima' := [solutieOptima[0],solutieOptima[1]-4,solutieOptima[2],solutieOptima[3],solutieOptima[4]];
+        assert esteSolutie(solutieOptima',copie-20);
+        assert cost(solutieOptima') == cost(solutieOptima)-4;
+        assert cost(solutieOptima)-4 < cost(solutieCurenta);
+        assert false;
+      }
+      else if(solutieOptima[1]>=3 && solutieOptima[0]>=5)
+      {
+        var solutieOptima' := [solutieOptima[0]-5,solutieOptima[1]-3,solutieOptima[2],solutieOptima[3],solutieOptima[4]];
+        assert esteSolutie(solutieOptima',copie-20);
+        assert cost(solutieOptima') == cost(solutieOptima)-8;
+        assert cost(solutieOptima)-8 < cost(solutieCurenta);
+        assert false;
+      }
+      else if(solutieOptima[1]>=2 && solutieOptima[0]>=10)
+      {
+        var solutieOptima' := [solutieOptima[0]-10,solutieOptima[1]-2,solutieOptima[2],solutieOptima[3],solutieOptima[4]];
+        assert esteSolutie(solutieOptima',copie-20);
+        assert cost(solutieOptima') == cost(solutieOptima)-12;
+        assert cost(solutieOptima)-12 < cost(solutieCurenta);
+        assert false;
+      }
+      else if(solutieOptima[1]>=1 && solutieOptima[0]>=15)
+      {
+        var solutieOptima' := [solutieOptima[0]-15,solutieOptima[1]-1,solutieOptima[2],solutieOptima[3],solutieOptima[4]];
+        assert esteSolutie(solutieOptima',copie-20);
+        assert cost(solutieOptima') == cost(solutieOptima)-16;
+        assert cost(solutieOptima)-16 < cost(solutieCurenta);
+        assert false;
+      }
+      else if(solutieOptima[0]>=20)
+      {
+        var solutieOptima' := [solutieOptima[0]-20,solutieOptima[1],solutieOptima[2],solutieOptima[3],solutieOptima[4]];
+        assert esteSolutie(solutieOptima',copie-20);
+        assert cost(solutieOptima') == cost(solutieOptima)-20;
+        assert cost(solutieOptima)-20 < cost(solutieCurenta);
+        assert false;
+      }
+      else if(solutieOptima[2]>=1 && solutieOptima[0]>=10)
+      {
+        var solutieOptima' := [solutieOptima[0]-10,solutieOptima[1],solutieOptima[2]-1,solutieOptima[3],solutieOptima[4]];
+        assert esteSolutie(solutieOptima',copie-20);
+        assert cost(solutieOptima') == cost(solutieOptima)-11;
+        assert cost(solutieOptima)-11 < cost(solutieCurenta);
+        assert false;
+      }
+      else{
+        assert false;
+      }
+    }
+
+}
+
+
+
+lemma cazMaxim20(copie: int, nr: int, solutieFinala: seq<int>)
+  requires 20 <= copie < 50 
+  requires esteSolutieValida(solutieFinala) 
+  requires INV(copie,nr,solutieFinala)
+  ensures INV(copie-20,nr,[solutieFinala[0],solutieFinala[1],solutieFinala[2],solutieFinala[3]+1,solutieFinala[4]])
+{
+
+ forall solutieCurenta | esteSolutieValida(solutieCurenta) && esteSolutieOptima(solutieCurenta,copie-20) 
+          ensures esteSolutieOptima([solutieFinala[0]+solutieCurenta[0],solutieFinala[1]+solutieCurenta[1],
+          solutieCurenta[2]+solutieFinala[2],solutieCurenta[3]+solutieFinala[3]+1,solutieCurenta[4]+solutieFinala[4]],nr)
+  {
+    assert esteSolutie(solutieCurenta,copie-20);
+    assert esteSolutie([solutieCurenta[0], solutieCurenta[1],solutieCurenta[2],solutieCurenta[3]+1,solutieCurenta[4]],copie);
+
+    aux3(copie,solutieCurenta);
+
+    assert esteSolutieOptima([solutieCurenta[0], solutieCurenta[1],solutieCurenta[2],1+solutieCurenta[3],solutieCurenta[4]],copie);
+
+    assert forall solutieOarecare :: esteSolutieValida(solutieOarecare)  && esteSolutie(solutieOarecare,copie-20) 
+          ==> cost(solutieOarecare) >= cost(solutieCurenta);
+    
+
+    assert esteSolutie([solutieFinala[0]+solutieCurenta[0],solutieFinala[1]+solutieCurenta[1],solutieFinala[2]+solutieCurenta[2],1+solutieFinala[3]+solutieCurenta[3],solutieFinala[4]+solutieCurenta[4]],nr);
+
+    assert forall solutieOarecare :: esteSolutieValida(solutieOarecare) && esteSolutie(solutieOarecare,nr)
+          ==> cost(solutieOarecare) >= cost([solutieCurenta[0]+solutieFinala[0],solutieCurenta[1]+solutieFinala[1],
+                                        solutieCurenta[2]+solutieFinala[2],1+solutieCurenta[3]+solutieFinala[3],solutieCurenta[4]+solutieFinala[4]]);
+  }
+
+  assert forall solutieCurenta :: esteSolutieValida(solutieCurenta) && esteSolutieOptima(solutieCurenta,copie-20) ==> 
+          esteSolutieOptima([solutieCurenta[0]+solutieFinala[0],solutieCurenta[1]+solutieFinala[1],
+                            solutieCurenta[2]+solutieFinala[2],1+solutieCurenta[3]+solutieFinala[3],solutieCurenta[4]+solutieFinala[4]],nr);
+
+}
+
 
 
 
 lemma B(copie:int,nr: int,solutieOarecare : seq<int>, solutieCurenta: seq<int>)
   requires esteSolutieValida(solutieOarecare)
   requires esteSolutieValida(solutieCurenta)
-  requires copie >= 20
+  requires copie >= 50
   requires esteSolutie(solutieOarecare,copie)
-  requires esteSolutie(solutieCurenta,copie-20)
-  requires esteSolutieOptima(solutieCurenta,copie-20)
-  ensures cost(solutieOarecare) >= cost([solutieCurenta[0],solutieCurenta[1],solutieCurenta[2],1+solutieCurenta[3]])
-  decreases solutieOarecare[0],solutieOarecare[1],solutieOarecare[2]
+  requires esteSolutie(solutieCurenta,copie-50)
+  requires esteSolutieOptima(solutieCurenta,copie-50)
+  ensures cost(solutieOarecare) >= cost([solutieCurenta[0],solutieCurenta[1],solutieCurenta[2],solutieCurenta[3],1+solutieCurenta[4]])
+  decreases solutieOarecare[0],solutieOarecare[1],solutieOarecare[2],solutieOarecare[3]
 {
   assert esteSolutie(solutieOarecare,copie);
-  assert esteSolutie([solutieCurenta[0],solutieCurenta[1],solutieCurenta[2],solutieCurenta[3]+1],copie);
+  assert esteSolutie([solutieCurenta[0],solutieCurenta[1],solutieCurenta[2],solutieCurenta[3],1+solutieCurenta[4]],copie);
 
-  if(cost(solutieOarecare) < cost([solutieCurenta[0],solutieCurenta[1],solutieCurenta[2],1+solutieCurenta[3]]))
+  if(cost(solutieOarecare) < cost([solutieCurenta[0],solutieCurenta[1],solutieCurenta[2],solutieCurenta[3],1+solutieCurenta[4]]))
   {
-    if(solutieOarecare[3] > (solutieCurenta[3]+1))
+    if(solutieOarecare[4] > solutieCurenta[4]+1)
     {
-      assert cost([solutieOarecare[0],solutieOarecare[1],solutieOarecare[2],solutieOarecare[3]-1]) < cost(solutieCurenta);
-      assert esteSolutieOptima([solutieOarecare[0],solutieOarecare[1],solutieOarecare[2],solutieOarecare[3]-1],(copie-20));
+      assert cost([solutieOarecare[0],solutieOarecare[1],solutieOarecare[2],solutieOarecare[3],solutieOarecare[4]-1]) < cost(solutieCurenta);
+      assert esteSolutieOptima([solutieOarecare[0],solutieOarecare[1],solutieOarecare[2],solutieOarecare[3],solutieOarecare[4]-1],(copie-50));
+      assert false;
+    }
+    else if(solutieOarecare[4]<solutieCurenta[4]+1)
+    {
+      assert (solutieOarecare[0]+(5*solutieOarecare[1])+(10*solutieOarecare[2])+(20*solutieOarecare[3]))>=50;
+
+      if(solutieOarecare[2]>=1 && solutieOarecare[3]>=2)
+      {
+          var nouaSolutieOarecare := [solutieOarecare[0],solutieOarecare[1],solutieOarecare[2]-1,solutieOarecare[3]-2,solutieOarecare[4]+1];
+          B(copie,nr,nouaSolutieOarecare, solutieCurenta);
+      }
+      else if(solutieOarecare[2]>=3 && solutieOarecare[3]>=1)
+      {
+          var nouaSolutieOarecare := [solutieOarecare[0],solutieOarecare[1],solutieOarecare[2]-3,solutieOarecare[3]-1,solutieOarecare[4]+1];
+          B(copie,nr,nouaSolutieOarecare, solutieCurenta);
+      }
+      else if(solutieOarecare[2]>=5)
+      {
+          var nouaSolutieOarecare := [solutieOarecare[0],solutieOarecare[1],solutieOarecare[2]-5,solutieOarecare[3],solutieOarecare[4]+1];
+          B(copie,nr,nouaSolutieOarecare, solutieCurenta);
+      }
+      else if(solutieOarecare[1]>=10)
+      {
+          var nouaSolutieOarecare := [solutieOarecare[0],solutieOarecare[1]-10,solutieOarecare[2],solutieOarecare[3],solutieOarecare[4]+1];
+          B(copie,nr,nouaSolutieOarecare, solutieCurenta);
+      }
+      else if(solutieOarecare[1]>=8 && solutieOarecare[2]>=1)
+      {
+          var nouaSolutieOarecare := [solutieOarecare[0],solutieOarecare[1]-8,solutieOarecare[2]-1,solutieOarecare[3],solutieOarecare[4]+1];
+          B(copie,nr,nouaSolutieOarecare, solutieCurenta);
+      }
+      else if(solutieOarecare[1]>=6 && solutieOarecare[2]>=2)
+      {
+          var nouaSolutieOarecare := [solutieOarecare[0],solutieOarecare[1]-6,solutieOarecare[2]-2,solutieOarecare[3],solutieOarecare[4]+1];
+          B(copie,nr,nouaSolutieOarecare, solutieCurenta);
+      }
+      else if(solutieOarecare[1]>=6 && solutieOarecare[3]>=1)
+      {
+          var nouaSolutieOarecare := [solutieOarecare[0],solutieOarecare[1]-6,solutieOarecare[2],solutieOarecare[3]-1,solutieOarecare[4]+1];
+          B(copie,nr,nouaSolutieOarecare, solutieCurenta);
+      }
+      else if(solutieOarecare[1]>=4 && solutieOarecare[2]>=3)
+      {
+          var nouaSolutieOarecare := [solutieOarecare[0],solutieOarecare[1]-4,solutieOarecare[2]-3,solutieOarecare[3],solutieOarecare[4]+1];
+          B(copie,nr,nouaSolutieOarecare, solutieCurenta);
+      }
+      else if(solutieOarecare[1]>=4 && solutieOarecare[2]>=1 && solutieOarecare[3]>=1)
+      {
+          var nouaSolutieOarecare := [solutieOarecare[0],solutieOarecare[1]-4,solutieOarecare[2]-1,solutieOarecare[3]-1,solutieOarecare[4]+1];
+          B(copie,nr,nouaSolutieOarecare, solutieCurenta);
+      }
+      else if(solutieOarecare[1]>=2 && solutieOarecare[2]>=4)
+      {
+          var nouaSolutieOarecare := [solutieOarecare[0],solutieOarecare[1]-2,solutieOarecare[2]-4,solutieOarecare[3],solutieOarecare[4]+1];
+          B(copie,nr,nouaSolutieOarecare, solutieCurenta);
+      }
+      else if(solutieOarecare[1]>=2 && solutieOarecare[2]>=2 && solutieOarecare[3]>=1)
+      {
+          var nouaSolutieOarecare := [solutieOarecare[0],solutieOarecare[1]-2,solutieOarecare[2]-2,solutieOarecare[3]-1,solutieOarecare[4]+1];
+          B(copie,nr,nouaSolutieOarecare, solutieCurenta);
+      }
+      else if(solutieOarecare[1]>=2 && solutieOarecare[3]>=2)
+      {
+          var nouaSolutieOarecare := [solutieOarecare[0],solutieOarecare[1]-2,solutieOarecare[2],solutieOarecare[3]-2,solutieOarecare[4]+1];
+          B(copie,nr,nouaSolutieOarecare, solutieCurenta);
+      }if(solutieOarecare[0]>=50)
+      {
+          var nouaSolutieOarecare := [solutieOarecare[0]-50,solutieOarecare[1],solutieOarecare[2],solutieOarecare[3],solutieOarecare[4]+1];
+          B(copie,nr,nouaSolutieOarecare, solutieCurenta);
+      }
+      else if(solutieOarecare[0]>=45 && solutieOarecare[1]>=1)
+      {
+          var nouaSolutieOarecare := [solutieOarecare[0]-45,solutieOarecare[1]-1,solutieOarecare[2],solutieOarecare[3],solutieOarecare[4]+1];
+          B(copie,nr,nouaSolutieOarecare, solutieCurenta);
+      }
+      else if(solutieOarecare[0]>=40 && solutieOarecare[1]>=2)
+      {
+          var nouaSolutieOarecare := [solutieOarecare[0]-40,solutieOarecare[1]-2,solutieOarecare[2],solutieOarecare[3],solutieOarecare[4]+1];
+          B(copie,nr,nouaSolutieOarecare, solutieCurenta);
+      }
+      else if(solutieOarecare[0]>=40 && solutieOarecare[2]>=1)
+      {
+          var nouaSolutieOarecare := [solutieOarecare[0]-40,solutieOarecare[1],solutieOarecare[2]-1,solutieOarecare[3],solutieOarecare[4]+1];
+          B(copie,nr,nouaSolutieOarecare, solutieCurenta);
+      }
+      else if(solutieOarecare[0]>=35 && solutieOarecare[1]>=3)
+      {
+          var nouaSolutieOarecare := [solutieOarecare[0]-35,solutieOarecare[1]-3,solutieOarecare[2],solutieOarecare[3],solutieOarecare[4]+1];
+          B(copie,nr,nouaSolutieOarecare, solutieCurenta);
+      }
+      else if(solutieOarecare[0]>=35 && solutieOarecare[1]>=1 &&solutieOarecare[2]>=1)
+      {
+          var nouaSolutieOarecare := [solutieOarecare[0]-35,solutieOarecare[1]-1,solutieOarecare[2]-1,solutieOarecare[3],solutieOarecare[4]+1];
+          B(copie,nr,nouaSolutieOarecare, solutieCurenta);
+      }
+      else if(solutieOarecare[0]>=30 && solutieOarecare[1]>=4)
+      {
+          var nouaSolutieOarecare := [solutieOarecare[0]-30,solutieOarecare[1]-4,solutieOarecare[2],solutieOarecare[3],solutieOarecare[4]+1];
+          B(copie,nr,nouaSolutieOarecare, solutieCurenta);
+      }
+      else if(solutieOarecare[0]>=30 && solutieOarecare[1]>=2 && solutieOarecare[2]>=1)
+      {
+          var nouaSolutieOarecare := [solutieOarecare[0]-30,solutieOarecare[1]-2,solutieOarecare[2]-1,solutieOarecare[3],solutieOarecare[4]+1];
+          B(copie,nr,nouaSolutieOarecare, solutieCurenta);
+      }
+      else if(solutieOarecare[0]>=30 && solutieOarecare[2]>=2)
+      {
+          var nouaSolutieOarecare := [solutieOarecare[0]-30,solutieOarecare[1],solutieOarecare[2]-2,solutieOarecare[3],solutieOarecare[4]+1];
+          B(copie,nr,nouaSolutieOarecare, solutieCurenta);
+      }
+      else if(solutieOarecare[0]>=30 && solutieOarecare[3]>=1)
+      {
+          var nouaSolutieOarecare := [solutieOarecare[0]-30,solutieOarecare[1],solutieOarecare[2],solutieOarecare[3]-1,solutieOarecare[4]+1];
+          B(copie,nr,nouaSolutieOarecare, solutieCurenta);
+      }
+      else if(solutieOarecare[0]>=25 && solutieOarecare[1]>=5)
+      {
+          var nouaSolutieOarecare := [solutieOarecare[0]-25,solutieOarecare[1]-5,solutieOarecare[2],solutieOarecare[3],solutieOarecare[4]+1];
+          B(copie,nr,nouaSolutieOarecare, solutieCurenta);
+      }
+      else if(solutieOarecare[0]>=25 && solutieOarecare[1]>=3 &&solutieOarecare[2]>=1)
+      {
+          var nouaSolutieOarecare := [solutieOarecare[0]-25,solutieOarecare[1]-3,solutieOarecare[2]-1,solutieOarecare[3],solutieOarecare[4]+1];
+          B(copie,nr,nouaSolutieOarecare, solutieCurenta);
+      }
+      else if(solutieOarecare[0]>=25 && solutieOarecare[1]>=1 &&solutieOarecare[2]>=2)
+      {
+          var nouaSolutieOarecare := [solutieOarecare[0]-25,solutieOarecare[1]-1,solutieOarecare[2]-2,solutieOarecare[3],solutieOarecare[4]+1];
+          B(copie,nr,nouaSolutieOarecare, solutieCurenta);
+      }
+      else if(solutieOarecare[0]>=25 && solutieOarecare[1]>=1 && solutieOarecare[3]>=1)
+      {
+          var nouaSolutieOarecare := [solutieOarecare[0]-25,solutieOarecare[1]-1,solutieOarecare[2],solutieOarecare[3]-1,solutieOarecare[4]+1];
+          B(copie,nr,nouaSolutieOarecare, solutieCurenta);
+      }
+      else if(solutieOarecare[0]>=20 && solutieOarecare[1]>=6)
+      {
+          var nouaSolutieOarecare := [solutieOarecare[0]-20,solutieOarecare[1]-6,solutieOarecare[2],solutieOarecare[3],solutieOarecare[4]+1];
+          B(copie,nr,nouaSolutieOarecare, solutieCurenta);
+      }
+      else if(solutieOarecare[0]>=20 && solutieOarecare[1]>=4 && solutieOarecare[2]>=1)
+      {
+          var nouaSolutieOarecare := [solutieOarecare[0]-20,solutieOarecare[1]-4,solutieOarecare[2]-1,solutieOarecare[3],solutieOarecare[4]+1];
+          B(copie,nr,nouaSolutieOarecare, solutieCurenta);
+      }
+      else if(solutieOarecare[0]>=20 && solutieOarecare[1]>=2 && solutieOarecare[2]>=2)
+      {
+          var nouaSolutieOarecare := [solutieOarecare[0]-20,solutieOarecare[1]-2,solutieOarecare[2]-2,solutieOarecare[3],solutieOarecare[4]+1];
+          B(copie,nr,nouaSolutieOarecare, solutieCurenta);
+      }
+      else if(solutieOarecare[0]>=20 && solutieOarecare[1]>=2 && solutieOarecare[3]>=1)
+      {
+          var nouaSolutieOarecare := [solutieOarecare[0]-20,solutieOarecare[1]-2,solutieOarecare[2],solutieOarecare[3]-1,solutieOarecare[4]+1];
+          B(copie,nr,nouaSolutieOarecare, solutieCurenta);
+      }
+      else if(solutieOarecare[0]>=20 && solutieOarecare[2]>=3)
+      {
+          var nouaSolutieOarecare := [solutieOarecare[0]-20,solutieOarecare[1],solutieOarecare[2]-3,solutieOarecare[3],solutieOarecare[4]+1];
+          B(copie,nr,nouaSolutieOarecare, solutieCurenta);
+      }
+      else if(solutieOarecare[0]>=20 && solutieOarecare[2]>=1 && solutieOarecare[3]>=1)
+      {
+          var nouaSolutieOarecare := [solutieOarecare[0]-20,solutieOarecare[1],solutieOarecare[2]-1,solutieOarecare[3]-1,solutieOarecare[4]+1];
+          B(copie,nr,nouaSolutieOarecare, solutieCurenta);
+      }
+      else if(solutieOarecare[0]>=15 && solutieOarecare[1]>=7)
+      {
+          var nouaSolutieOarecare := [solutieOarecare[0]-15,solutieOarecare[1]-7,solutieOarecare[2],solutieOarecare[3],solutieOarecare[4]+1];
+          B(copie,nr,nouaSolutieOarecare, solutieCurenta);
+      }
+      else if(solutieOarecare[0]>=15 && solutieOarecare[1]>=5 && solutieOarecare[2]>=1)
+      {
+          var nouaSolutieOarecare := [solutieOarecare[0]-15,solutieOarecare[1]-5,solutieOarecare[2]-1,solutieOarecare[3],solutieOarecare[4]+1];
+          B(copie,nr,nouaSolutieOarecare, solutieCurenta);
+      }
+      else if(solutieOarecare[0]>=15 && solutieOarecare[1]>=3 && solutieOarecare[2]>=2)
+      {
+          var nouaSolutieOarecare := [solutieOarecare[0]-15,solutieOarecare[1]-3,solutieOarecare[2]-2,solutieOarecare[3],solutieOarecare[4]+1];
+          B(copie,nr,nouaSolutieOarecare, solutieCurenta);
+      }
+      else if(solutieOarecare[0]>=15 && solutieOarecare[1]>=3 && solutieOarecare[3]>=1)
+      {
+          var nouaSolutieOarecare := [solutieOarecare[0]-15,solutieOarecare[1]-3,solutieOarecare[2],solutieOarecare[3]-1,solutieOarecare[4]+1];
+          B(copie,nr,nouaSolutieOarecare, solutieCurenta);
+      }
+      else if(solutieOarecare[0]>=15 && solutieOarecare[1]>=1 && solutieOarecare[2]>=3)
+      {
+          var nouaSolutieOarecare := [solutieOarecare[0]-15,solutieOarecare[1]-1,solutieOarecare[2]-3,solutieOarecare[3],solutieOarecare[4]+1];
+          B(copie,nr,nouaSolutieOarecare, solutieCurenta);
+      }
+      else if(solutieOarecare[0]>=15 && solutieOarecare[1]>=1 && solutieOarecare[2]>=1 && solutieOarecare[3]>=1)
+      {
+          var nouaSolutieOarecare := [solutieOarecare[0]-15,solutieOarecare[1]-1,solutieOarecare[2]-1,solutieOarecare[3]-1,solutieOarecare[4]+1];
+          B(copie,nr,nouaSolutieOarecare, solutieCurenta);
+      }
+      else if(solutieOarecare[0]>=10 && solutieOarecare[1]>=8)
+      {
+          var nouaSolutieOarecare := [solutieOarecare[0]-10,solutieOarecare[1]-8,solutieOarecare[2],solutieOarecare[3],solutieOarecare[4]+1];
+          B(copie,nr,nouaSolutieOarecare, solutieCurenta);
+      }
+      else if(solutieOarecare[0]>=10 && solutieOarecare[1]>=6 && solutieOarecare[2]>=1)
+      {
+          var nouaSolutieOarecare := [solutieOarecare[0]-10,solutieOarecare[1]-6,solutieOarecare[2]-1,solutieOarecare[3],solutieOarecare[4]+1];
+          B(copie,nr,nouaSolutieOarecare, solutieCurenta);
+      }
+      else if(solutieOarecare[0]>=10 && solutieOarecare[1]>=4 && solutieOarecare[2]>=2)
+      {
+          var nouaSolutieOarecare := [solutieOarecare[0]-10,solutieOarecare[1]-4,solutieOarecare[2]-2,solutieOarecare[3],solutieOarecare[4]+1];
+          B(copie,nr,nouaSolutieOarecare, solutieCurenta);
+      }
+      else if(solutieOarecare[0]>=10 && solutieOarecare[1]>=4 && solutieOarecare[3]>=1)
+      {
+          var nouaSolutieOarecare := [solutieOarecare[0]-10,solutieOarecare[1]-4,solutieOarecare[2],solutieOarecare[3]-1,solutieOarecare[4]+1];
+          B(copie,nr,nouaSolutieOarecare, solutieCurenta);
+      }
+      else if(solutieOarecare[0]>=10 && solutieOarecare[1]>=2 && solutieOarecare[2]>=3)
+      {
+          var nouaSolutieOarecare := [solutieOarecare[0]-10,solutieOarecare[1]-2,solutieOarecare[2]-3,solutieOarecare[3],solutieOarecare[4]+1];
+          B(copie,nr,nouaSolutieOarecare, solutieCurenta);
+      }
+      else if(solutieOarecare[0]>=10 && solutieOarecare[1]>=2 && solutieOarecare[2]>=1 && solutieOarecare[3]>=1)
+      {
+          var nouaSolutieOarecare := [solutieOarecare[0]-10,solutieOarecare[1]-2,solutieOarecare[2]-1,solutieOarecare[3]-1,solutieOarecare[4]+1];
+          B(copie,nr,nouaSolutieOarecare, solutieCurenta);
+      }
+      else if(solutieOarecare[0]>=10 && solutieOarecare[2]>=4)
+      {
+          var nouaSolutieOarecare := [solutieOarecare[0]-10,solutieOarecare[1],solutieOarecare[2]-4,solutieOarecare[3],solutieOarecare[4]+1];
+          B(copie,nr,nouaSolutieOarecare, solutieCurenta);
+      }
+      else if(solutieOarecare[0]>=10 && solutieOarecare[2]>=2 && solutieOarecare[3]>=1)
+      {
+          var nouaSolutieOarecare := [solutieOarecare[0]-10,solutieOarecare[1],solutieOarecare[2]-2,solutieOarecare[3]-1,solutieOarecare[4]+1];
+          B(copie,nr,nouaSolutieOarecare, solutieCurenta);
+      }
+      else if(solutieOarecare[0]>=10 && solutieOarecare[3]>=2)
+      {
+          var nouaSolutieOarecare := [solutieOarecare[0]-10,solutieOarecare[1],solutieOarecare[2],solutieOarecare[3]-2,solutieOarecare[4]+1];
+          B(copie,nr,nouaSolutieOarecare, solutieCurenta);
+      }
+      else if(solutieOarecare[0]>=5 && solutieOarecare[1]>=9)
+      {
+          var nouaSolutieOarecare := [solutieOarecare[0]-5,solutieOarecare[1]-9,solutieOarecare[2],solutieOarecare[3],solutieOarecare[4]+1];
+          B(copie,nr,nouaSolutieOarecare, solutieCurenta);
+      }
+      else if(solutieOarecare[0]>=5 && solutieOarecare[1]>=7 && solutieOarecare[2]>=1)
+      {
+          var nouaSolutieOarecare := [solutieOarecare[0]-5,solutieOarecare[1]-7,solutieOarecare[2]-1,solutieOarecare[3],solutieOarecare[4]+1];
+          B(copie,nr,nouaSolutieOarecare, solutieCurenta);
+      }
+      else if(solutieOarecare[0]>=5 && solutieOarecare[1]>=5 && solutieOarecare[2]>=2)
+      {
+          var nouaSolutieOarecare := [solutieOarecare[0]-5,solutieOarecare[1]-5,solutieOarecare[2]-2,solutieOarecare[3],solutieOarecare[4]+1];
+          B(copie,nr,nouaSolutieOarecare, solutieCurenta);
+      }
+      else if(solutieOarecare[0]>=5 && solutieOarecare[1]>=5 && solutieOarecare[3]>=1)
+      {
+          var nouaSolutieOarecare := [solutieOarecare[0]-5,solutieOarecare[1]-5,solutieOarecare[2],solutieOarecare[3]-1,solutieOarecare[4]+1];
+          B(copie,nr,nouaSolutieOarecare, solutieCurenta);
+      }
+      else if(solutieOarecare[0]>=5 && solutieOarecare[1]>=3 && solutieOarecare[2]>=3)
+      {
+          var nouaSolutieOarecare := [solutieOarecare[0]-5,solutieOarecare[1]-3,solutieOarecare[2]-3,solutieOarecare[3],solutieOarecare[4]+1];
+          B(copie,nr,nouaSolutieOarecare, solutieCurenta);
+      }
+      else if(solutieOarecare[0]>=5 && solutieOarecare[1]>=3 && solutieOarecare[2]>=1 && solutieOarecare[3]>=1)
+      {
+          var nouaSolutieOarecare := [solutieOarecare[0]-5,solutieOarecare[1]-3,solutieOarecare[2]-1,solutieOarecare[3]-1,solutieOarecare[4]+1];
+          B(copie,nr,nouaSolutieOarecare, solutieCurenta);
+      }
+      else if(solutieOarecare[0]>=5 && solutieOarecare[1]>=1 && solutieOarecare[2]>=4)
+      {
+          var nouaSolutieOarecare := [solutieOarecare[0]-5,solutieOarecare[1]-1,solutieOarecare[2]-4,solutieOarecare[3],solutieOarecare[4]+1];
+          B(copie,nr,nouaSolutieOarecare, solutieCurenta);
+      }
+      else if(solutieOarecare[0]>=5 && solutieOarecare[1]>=1 && solutieOarecare[2]>=2 && solutieOarecare[3]>=1)
+      {
+          var nouaSolutieOarecare := [solutieOarecare[0]-5,solutieOarecare[1]-1,solutieOarecare[2]-2,solutieOarecare[3]-1,solutieOarecare[4]+1];
+          B(copie,nr,nouaSolutieOarecare, solutieCurenta);
+      }
+      else if(solutieOarecare[0]>=5 && solutieOarecare[1]>=1 && solutieOarecare[3]>=2)
+      {
+          var nouaSolutieOarecare := [solutieOarecare[0]-5,solutieOarecare[1]-1,solutieOarecare[2],solutieOarecare[3]-2,solutieOarecare[4]+1];
+          B(copie,nr,nouaSolutieOarecare, solutieCurenta);
+      }
+      else{
+          
+          assert solutieOarecare[0]>=0;
+          assert solutieOarecare[1]>=0;
+          assert solutieOarecare[2]>=0;
+          assert solutieOarecare[3]>=3;
+          if(solutieOarecare[3]>=5)
+          {
+            var nouaSolutieOarecare := [solutieOarecare[0],solutieOarecare[1],solutieOarecare[2],solutieOarecare[3]-5,solutieOarecare[4]+2];
+            assert cost(nouaSolutieOarecare) < cost(solutieOarecare);
+            B(copie, nr, nouaSolutieOarecare, solutieCurenta);
+          }
+      }
+
+      
+    }
+    
+    assert solutieOarecare[4]==(solutieCurenta[4]+1);
+
+
+    if(solutieOarecare[3] > solutieCurenta[3])
+    {
+      assert cost([solutieOarecare[0],solutieOarecare[1],solutieOarecare[2],solutieOarecare[3],solutieOarecare[4]-1]) < cost(solutieCurenta);
       assert false;
       
     }
-    else if(solutieOarecare[3] < solutieCurenta[3]+1)
+    else if(solutieOarecare[3] < solutieCurenta[3])
       {
         assert (solutieOarecare[0]+(5*solutieOarecare[1])+(10*solutieOarecare[2]))>20;
         
         if(solutieOarecare[2]>=2)
         {
-            var nouaSolutieOarecare := [solutieOarecare[0],solutieOarecare[1],solutieOarecare[2]-2,solutieOarecare[3]+1];
+            assert solutieOarecare[2]>=2;
+            var nouaSolutieOarecare := [solutieOarecare[0],solutieOarecare[1],solutieOarecare[2]-2,solutieOarecare[3]+1,solutieOarecare[4]];
             B(copie,nr,nouaSolutieOarecare, solutieCurenta);
         }
         else if(solutieOarecare[2]>=1 && solutieOarecare[1]>=2)
         {
-            var nouaSolutieOarecare := [solutieOarecare[0],solutieOarecare[1]-2,solutieOarecare[2]-1,solutieOarecare[3]+1];
+            var nouaSolutieOarecare := [solutieOarecare[0],solutieOarecare[1]-2,solutieOarecare[2]-1,solutieOarecare[3]+1,solutieOarecare[4]];
             B(copie,nr,nouaSolutieOarecare, solutieCurenta);
         }
         else if(solutieOarecare[2]>=1 && solutieOarecare[1]>=1 && solutieOarecare[0]>=5)
         {
-            var nouaSolutieOarecare := [solutieOarecare[0]-5,solutieOarecare[1]-1,solutieOarecare[2]-1,solutieOarecare[3]+1];
+            var nouaSolutieOarecare := [solutieOarecare[0]-5,solutieOarecare[1]-1,solutieOarecare[2]-1,solutieOarecare[3]+1,solutieOarecare[4]];
             B(copie,nr,nouaSolutieOarecare, solutieCurenta);
         }
         else if(solutieOarecare[1]>=4)
         {
-            var nouaSolutieOarecare := [solutieOarecare[0],solutieOarecare[1]-4,solutieOarecare[2],solutieOarecare[3]+1];
+            var nouaSolutieOarecare := [solutieOarecare[0],solutieOarecare[1]-4,solutieOarecare[2],solutieOarecare[3]+1,solutieOarecare[4]];
             B(copie,nr,nouaSolutieOarecare, solutieCurenta);
         }
         else if(solutieOarecare[1]>=3 && solutieOarecare[0]>=5)
         {
-            var nouaSolutieOarecare := [solutieOarecare[0]-5,solutieOarecare[1]-3,solutieOarecare[2],solutieOarecare[3]+1];
+            var nouaSolutieOarecare := [solutieOarecare[0]-5,solutieOarecare[1]-3,solutieOarecare[2],solutieOarecare[3]+1,solutieOarecare[4]];
             B(copie,nr,nouaSolutieOarecare, solutieCurenta);
         }
         else if(solutieOarecare[1]>=2 && solutieOarecare[0]>=10)
         {
-            var nouaSolutieOarecare := [solutieOarecare[0]-10,solutieOarecare[1]-2,solutieOarecare[2],solutieOarecare[3]+1];
+            var nouaSolutieOarecare := [solutieOarecare[0]-10,solutieOarecare[1]-2,solutieOarecare[2],solutieOarecare[3]+1,solutieOarecare[4]];
             B(copie,nr,nouaSolutieOarecare, solutieCurenta);
         }
         else if(solutieOarecare[1]>=1 && solutieOarecare[0]>=15)
         {
-          var nouaSolutieOarecare := [solutieOarecare[0]-15,solutieOarecare[1]-1,solutieOarecare[2],solutieOarecare[3]+1];
+          var nouaSolutieOarecare := [solutieOarecare[0]-15,solutieOarecare[1]-1,solutieOarecare[2],solutieOarecare[3]+1,solutieOarecare[4]];
             B(copie,nr,nouaSolutieOarecare, solutieCurenta);
         }
         else if(solutieOarecare[0]>=20)
         {
-            var nouaSolutieOarecare := [solutieOarecare[0]-20,solutieOarecare[1],solutieOarecare[2],solutieOarecare[3]+1];
+            var nouaSolutieOarecare := [solutieOarecare[0]-20,solutieOarecare[1],solutieOarecare[2],solutieOarecare[3]+1,solutieOarecare[4]];
             B(copie,nr,nouaSolutieOarecare, solutieCurenta);
         }
         else if(solutieOarecare[2]>=1 && solutieOarecare[0]>=10)
         {
-            var nouaSolutieOarecare := [solutieOarecare[0]-10,solutieOarecare[1],solutieOarecare[2]-1,solutieOarecare[3]+1];
+            var nouaSolutieOarecare := [solutieOarecare[0]-10,solutieOarecare[1],solutieOarecare[2]-1,solutieOarecare[3]+1,solutieOarecare[4]];
             B(copie,nr,nouaSolutieOarecare, solutieCurenta);
         }
       }
 
-    assert solutieOarecare[3] == (solutieCurenta[3]+1);
+    assert solutieOarecare[3] == solutieCurenta[3];
 
     if(solutieOarecare[2]>solutieCurenta[2])
     {
-      assert cost([solutieOarecare[0],solutieOarecare[1],solutieOarecare[2],solutieOarecare[3]-1]) < cost(solutieCurenta);
+      assert cost([solutieOarecare[0],solutieOarecare[1],solutieOarecare[2],solutieOarecare[3],solutieOarecare[4]-1]) < cost(solutieCurenta);
       assert false;
     }
     else if(solutieOarecare[2] < solutieCurenta[2])
@@ -303,16 +761,16 @@ lemma B(copie:int,nr: int,solutieOarecare : seq<int>, solutieCurenta: seq<int>)
 
         if(solutieOarecare[0]>=10)
         {
-          var nouaSolutieOarecare := [solutieOarecare[0]-10,solutieOarecare[1],solutieOarecare[2]+1,solutieOarecare[3]];
+          var nouaSolutieOarecare := [solutieOarecare[0]-10,solutieOarecare[1],solutieOarecare[2]+1,solutieOarecare[3],solutieOarecare[4]];
           B(copie,nr,nouaSolutieOarecare, solutieCurenta);
         }
         else if(solutieOarecare[1]>=2){
-            var nouaSolutieOarecare := [solutieOarecare[0],solutieOarecare[1]-2,solutieOarecare[2]+1,solutieOarecare[3]];
+            var nouaSolutieOarecare := [solutieOarecare[0],solutieOarecare[1]-2,solutieOarecare[2]+1,solutieOarecare[3],solutieOarecare[4]];
              B(copie,nr,nouaSolutieOarecare, solutieCurenta);
         }
           else
           {
-            var nouaSolutieOarecare := [solutieOarecare[0]-5,solutieOarecare[1]-1,solutieOarecare[2]+1,solutieOarecare[3]];
+            var nouaSolutieOarecare := [solutieOarecare[0]-5,solutieOarecare[1]-1,solutieOarecare[2]+1,solutieOarecare[3],solutieOarecare[4]];
              B(copie,nr,nouaSolutieOarecare, solutieCurenta);
           }
         }
@@ -320,16 +778,15 @@ lemma B(copie:int,nr: int,solutieOarecare : seq<int>, solutieCurenta: seq<int>)
 
       if(solutieOarecare[1]>solutieCurenta[1])
     {
-      assert cost([solutieOarecare[0],solutieOarecare[1],solutieOarecare[2],solutieOarecare[3]-1]) < cost(solutieCurenta);
+      assert cost([solutieOarecare[0],solutieOarecare[1],solutieOarecare[2],solutieOarecare[3],solutieOarecare[4]-1]) < cost(solutieCurenta);
       assert false;
     }
     else
     {
       if(solutieOarecare[1]<solutieCurenta[1])
       {
-        assert solutieOarecare[0]>=5;
-      
-          var nouaSolutieOarecare := [solutieOarecare[0]-5,solutieOarecare[1]+1,solutieOarecare[2],solutieOarecare[3]];
+          assert solutieOarecare[0]>=5;
+          var nouaSolutieOarecare := [solutieOarecare[0]-5,solutieOarecare[1]+1,solutieOarecare[2],solutieOarecare[3],solutieOarecare[4]];
           B(copie, nr, nouaSolutieOarecare, solutieCurenta);
         
       }
@@ -342,13 +799,13 @@ lemma B(copie:int,nr: int,solutieOarecare : seq<int>, solutieCurenta: seq<int>)
 
 lemma esteSolutiePentruCopie(copie:int,nr: int, solutieCurenta:seq<int>)
   requires esteSolutieValida(solutieCurenta)
-  requires copie >= 20
-  requires esteSolutie(solutieCurenta,copie-20)
-  requires esteSolutieOptima(solutieCurenta,copie-20)
-  ensures esteSolutieOptima([solutieCurenta[0],solutieCurenta[1],solutieCurenta[2],1+solutieCurenta[3]],copie)
+  requires copie >= 50
+  requires esteSolutie(solutieCurenta,copie-50)
+  requires esteSolutieOptima(solutieCurenta,copie-50)
+  ensures esteSolutieOptima([solutieCurenta[0],solutieCurenta[1],solutieCurenta[2],solutieCurenta[3],1+solutieCurenta[4]],copie)
 {
   forall solutieOarecare | esteSolutieValida(solutieOarecare) && esteSolutie(solutieOarecare,copie)
-    ensures cost(solutieOarecare)>=cost([solutieCurenta[0],solutieCurenta[1],solutieCurenta[2],1+solutieCurenta[3]])
+    ensures cost(solutieOarecare)>=cost([solutieCurenta[0],solutieCurenta[1],solutieCurenta[2],solutieCurenta[3],1+solutieCurenta[4]])
   {
     B(copie,nr, solutieOarecare, solutieCurenta);
   }
@@ -359,12 +816,12 @@ lemma aux(copie: int ,nr: int, solutieOarecare : seq<int>, solutieFinala : seq<i
   requires esteSolutieValida(solutieOarecare)
   requires esteSolutieValida(solutieFinala)
   requires esteSolutieValida(solutieCurenta)
-  requires copie >= 20
-  requires esteSolutieOptima(solutieCurenta,copie-20)
-  requires esteSolutie([solutieFinala[0]+solutieCurenta[0],solutieFinala[1]+solutieCurenta[1],solutieFinala[2]+solutieCurenta[2],1+solutieFinala[3]+solutieCurenta[3]],nr)
+  requires copie >= 50
+  requires esteSolutieOptima(solutieCurenta,copie-50)
+  requires esteSolutie([solutieFinala[0]+solutieCurenta[0],solutieFinala[1]+solutieCurenta[1],solutieFinala[2]+solutieCurenta[2],solutieFinala[3]+solutieCurenta[3],1+solutieFinala[4]+solutieCurenta[4]],nr)
   requires esteSolutie(solutieOarecare,nr)
   requires INV(copie,nr,solutieFinala)
-  ensures cost(solutieOarecare) >= cost([solutieFinala[0]+solutieCurenta[0],solutieFinala[1]+solutieCurenta[1],solutieFinala[2]+solutieCurenta[2],1+solutieFinala[3]+solutieCurenta[3]])
+  ensures cost(solutieOarecare) >= cost([solutieFinala[0]+solutieCurenta[0],solutieFinala[1]+solutieCurenta[1],solutieFinala[2]+solutieCurenta[2],solutieFinala[3]+solutieCurenta[3],1+solutieFinala[4]+solutieCurenta[4]])
 {
   esteSolutiePentruCopie(copie,nr,solutieCurenta);
 }
@@ -372,66 +829,66 @@ lemma aux(copie: int ,nr: int, solutieOarecare : seq<int>, solutieFinala : seq<i
 
 
 
-lemma cazMaxim20(copie: int,nr: int, solutieFinala : seq<int>)
-  requires copie >= 20
+lemma cazMaxim50(copie: int,nr: int, solutieFinala : seq<int>)
+  requires copie >= 50
   requires esteSolutieValida(solutieFinala)
   requires INV(copie,nr,solutieFinala)
-  ensures INV(copie-20,nr,[solutieFinala[0],solutieFinala[1],solutieFinala[2],solutieFinala[3]+1])
+  ensures INV(copie-50,nr,[solutieFinala[0],solutieFinala[1],solutieFinala[2],solutieFinala[3],1+solutieFinala[4]])
 {
   assert forall solutieCurenta :: esteSolutieValida(solutieCurenta) ==>
           (esteSolutie(solutieCurenta,copie) ==> 
-          esteSolutie([solutieFinala[0]+solutieCurenta[0],solutieFinala[1]+solutieCurenta[1],solutieFinala[2]+solutieCurenta[2],solutieFinala[3]+solutieCurenta[3]],nr));
+          esteSolutie([solutieFinala[0]+solutieCurenta[0],solutieFinala[1]+solutieCurenta[1],solutieFinala[2]+solutieCurenta[2],solutieFinala[3]+solutieCurenta[3],solutieFinala[4]+solutieCurenta[4]],nr));
 
    forall solutieCurenta | esteSolutieValida(solutieCurenta) 
-          && esteSolutie(solutieCurenta,copie-20) 
-          ensures esteSolutie([solutieFinala[0]+solutieCurenta[0],solutieFinala[1]+solutieCurenta[1],solutieFinala[2]+solutieCurenta[2],solutieFinala[3]+solutieCurenta[3]+1],nr)
+          && esteSolutie(solutieCurenta,copie-50) 
+          ensures esteSolutie([solutieFinala[0]+solutieCurenta[0],solutieFinala[1]+solutieCurenta[1],solutieFinala[2]+solutieCurenta[2],solutieFinala[3]+solutieCurenta[3],1+solutieFinala[4]+solutieCurenta[4]],nr)
    {
-     assert esteSolutie([solutieCurenta[0],solutieCurenta[1],solutieCurenta[2],solutieCurenta[3]+1],copie);
+     assert esteSolutie([solutieCurenta[0],solutieCurenta[1],solutieCurenta[2],solutieCurenta[3],1+solutieCurenta[4]],copie);
    }
   
 
   forall solutieCurenta | esteSolutieValida(solutieCurenta) 
-          && esteSolutieOptima(solutieCurenta,copie-20) 
-          ensures esteSolutieOptima([solutieFinala[0]+solutieCurenta[0],solutieFinala[1]+solutieCurenta[1],solutieFinala[2]+solutieCurenta[2],solutieFinala[3]+solutieCurenta[3]+1],nr)
+          && esteSolutieOptima(solutieCurenta,copie-50) 
+          ensures esteSolutieOptima([solutieFinala[0]+solutieCurenta[0],solutieFinala[1]+solutieCurenta[1],solutieFinala[2]+solutieCurenta[2],solutieFinala[3]+solutieCurenta[3],1+solutieFinala[4]+solutieCurenta[4]],nr)
   {
 
-    assert esteSolutie(solutieCurenta,copie-20);
-    assert esteSolutie([solutieCurenta[0],solutieCurenta[1],solutieCurenta[2],solutieCurenta[3]+1],copie);
+    assert esteSolutie(solutieCurenta,copie-50);
+    assert esteSolutie([solutieCurenta[0],solutieCurenta[1],solutieCurenta[2],solutieCurenta[3],1+solutieCurenta[4]],copie);
 
     assert forall solutieOarecare :: esteSolutieValida(solutieOarecare)
-          && esteSolutie(solutieOarecare,copie-20) 
+          && esteSolutie(solutieOarecare,copie-50) 
           ==> cost(solutieOarecare) >= cost(solutieCurenta);
 
 
-    assert esteSolutie([solutieFinala[0]+solutieCurenta[0],solutieFinala[1]+solutieCurenta[1],solutieFinala[2]+solutieCurenta[2],solutieFinala[3]+solutieCurenta[3]+1],nr);
+    assert esteSolutie([solutieFinala[0]+solutieCurenta[0],solutieFinala[1]+solutieCurenta[1],solutieFinala[2]+solutieCurenta[2],solutieFinala[3]+solutieCurenta[3],1+solutieFinala[4]+solutieCurenta[4]],nr);
 
     forall solutieOarecare | esteSolutieValida(solutieOarecare)
                  && esteSolutie(solutieOarecare,nr)
-      ensures cost(solutieOarecare) >= cost([solutieFinala[0]+solutieCurenta[0],solutieFinala[1]+solutieCurenta[1],solutieFinala[2]+solutieCurenta[2],1+solutieFinala[3]+solutieCurenta[3]])
+      ensures cost(solutieOarecare) >= cost([solutieFinala[0]+solutieCurenta[0],solutieFinala[1]+solutieCurenta[1],solutieFinala[2]+solutieCurenta[2],solutieFinala[3]+solutieCurenta[3],1+solutieFinala[4]+solutieCurenta[4]])
       {
           aux(copie, nr, solutieOarecare, solutieFinala, solutieCurenta);
       }
 
     assert forall solutieOarecare :: esteSolutieValida(solutieOarecare)
              && esteSolutie(solutieOarecare,nr) 
-          ==> cost(solutieOarecare) >= cost([solutieFinala[0]+solutieCurenta[0],solutieFinala[1]+solutieCurenta[1],solutieFinala[2]+solutieCurenta[2],1+solutieFinala[3]+solutieCurenta[3]]);
+          ==> cost(solutieOarecare) >= cost([solutieFinala[0]+solutieCurenta[0],solutieFinala[1]+solutieCurenta[1],solutieFinala[2]+solutieCurenta[2],solutieFinala[3]+solutieCurenta[3],1+solutieFinala[4]+solutieCurenta[4]]);
   }
 
 
   assert forall solutieCurenta :: esteSolutieValida(solutieCurenta)
-          && esteSolutieOptima(solutieCurenta,copie-20) ==> 
-          esteSolutieOptima([solutieFinala[0]+solutieCurenta[0],solutieFinala[1]+solutieCurenta[1],solutieFinala[2]+solutieCurenta[2],1+solutieFinala[3]+solutieCurenta[3]],nr);
+          && esteSolutieOptima(solutieCurenta,copie-50) ==> 
+          esteSolutieOptima([solutieFinala[0]+solutieCurenta[0],solutieFinala[1]+solutieCurenta[1],solutieFinala[2]+solutieCurenta[2],solutieFinala[3]+solutieCurenta[3],1+solutieFinala[4]+solutieCurenta[4]],nr);
 
 
   assert forall solutieCurenta :: esteSolutieValida(solutieCurenta) ==>
-          (esteSolutie(solutieCurenta,copie-20) ==> 
-          esteSolutie([solutieFinala[0]+solutieCurenta[0],solutieFinala[1]+solutieCurenta[1],solutieFinala[2]+solutieCurenta[2],1+solutieFinala[3]+solutieCurenta[3]],nr));
+          (esteSolutie(solutieCurenta,copie-50) ==> 
+          esteSolutie([solutieFinala[0]+solutieCurenta[0],solutieFinala[1]+solutieCurenta[1],solutieFinala[2]+solutieCurenta[2],solutieFinala[3]+solutieCurenta[3],1+solutieFinala[4]+solutieCurenta[4]],nr));
   
   assert forall solutieCurenta :: esteSolutieValida(solutieCurenta) ==>        
-          (esteSolutieOptima(solutieCurenta,copie-20) ==> 
-          esteSolutieOptima([solutieFinala[0]+solutieCurenta[0],solutieFinala[1]+solutieCurenta[1],solutieFinala[2]+solutieCurenta[2],solutieFinala[3]+solutieCurenta[3]+1],nr));
+          (esteSolutieOptima(solutieCurenta,copie-50) ==> 
+          esteSolutieOptima([solutieFinala[0]+solutieCurenta[0],solutieFinala[1]+solutieCurenta[1],solutieFinala[2]+solutieCurenta[2],solutieFinala[3]+solutieCurenta[3],1+solutieFinala[4]+solutieCurenta[4]],nr));
 
-  assert  INV(copie-20,nr,[solutieFinala[0],solutieFinala[1],solutieFinala[2],1+solutieFinala[3]]);
+  assert  INV(copie-50,nr,[solutieFinala[0],solutieFinala[1],solutieFinala[2],solutieFinala[3],1+solutieFinala[4]]);
 }
 
 
@@ -448,45 +905,53 @@ lemma cazMaxim20(copie: int,nr: int, solutieFinala : seq<int>)
     var s5 := 0;
     var s10 := 0;
     var s20 := 0;
+    var s50 := 0;
     while(copie > 0)
       decreases copie
       invariant 0<=copie<=nr
-      invariant esteSolutie([s1,s5,s10,s20],nr-copie)
-      invariant INV(copie,nr,[s1,s5,s10,s20])
+      invariant esteSolutie([s1,s5,s10,s20,s50],nr-copie)
+      invariant INV(copie,nr,[s1,s5,s10,s20,s50])
     {
         var i := 0;
         var s := gasireMaxim(copie);
         if( s == 1){
-            cazMaxim1(copie,nr,[s1,s5,s10,s20]);
+            cazMaxim1(copie,nr,[s1,s5,s10,s20,s50]);
             s1:=s1+1;
-            assert esteSolutie([s1,s5,s10,s20],nr-(copie-1));
-            assert INV(copie-1,nr,[s1,s5,s10,s20]);
+            assert esteSolutie([s1,s5,s10,s20,s50],nr-(copie-1));
+            assert INV(copie-1,nr,[s1,s5,s10,s20,s50]);
         }
         else if(s == 5)
             {
-                cazMaxim5(copie,nr,[s1,s5,s10,s20]);
+                cazMaxim5(copie,nr,[s1,s5,s10,s20,s50]);
                 s5:=s5+1;
-                assert esteSolutie([s1,s5,s10,s20],nr-(copie-5));
-                assert INV(copie-5,nr,[s1,s5,s10,s20]);
+                assert esteSolutie([s1,s5,s10,s20,s50],nr-(copie-5));
+                assert INV(copie-5,nr,[s1,s5,s10,s20,s50]);
 
             }
             else if (s == 10){
-                cazMaxim10(copie,nr,[s1,s5,s10,s20]);
+                cazMaxim10(copie,nr,[s1,s5,s10,s20,s50]);
                 s10:=s10+1;
-                assert esteSolutie([s1,s5,s10,s20],nr-(copie-10));
-                assert INV(copie-10,nr,[s1,s5,s10,s20]);
+                assert esteSolutie([s1,s5,s10,s20,s50],nr-(copie-10));
+                assert INV(copie-10,nr,[s1,s5,s10,s20,s50]);
 
             }
-            else{
-                cazMaxim20(copie,nr,[s1,s5,s10,s20]);
+            else if(s == 20){
+                cazMaxim20(copie,nr,[s1,s5,s10,s20,s50]);
                 s20:=s20+1;
-                assert esteSolutie([s1,s5,s10,s20],nr-(copie-20));
-                assert INV(copie-20,nr,[s1,s5,s10,s20]);
+                assert esteSolutie([s1,s5,s10,s20,s50],nr-(copie-20));
+                assert INV(copie-20,nr,[s1,s5,s10,s20,s50]);
+            }
+            else{
+                // cazMaxim50(copie,nr,[s1,s5,s10,s20,s50]);
+                // s50:=s50+1;
+                // assert esteSolutie([s1,s5,s10,s20,s50],nr-(copie-50));
+                // assert INV(copie-50,nr,[s1,s5,s10,s20,s50]);
+                assume false;
             }
 
         copie := copie-s;
     }
-    solutie := [s1,s5,s10,s20];
+    solutie := [s1,s5,s10,s20,s50];
 }
 
 
